feat: add more attributes to encryption context (#719)
* feat: add more attributes to encryption context

DynamoDbEncryption/runtimes/java/src/main/java/software/amazon/cryptography/dbencryptionsdk/dynamodb/enhancedclient/DynamoDbEnhancedClientEncryption.java
@@ -4,6 +4,7 @@ import java.util.Collections;
 import java.util.HashMap;
 import java.util.HashSet;
 import java.util.List;
+import java.util.ArrayList;
 import java.util.Map;
 import java.util.Objects;
 import java.util.Optional;
@@ -24,6 +25,7 @@ import software.amazon.cryptography.dbencryptionsdk.structuredencryption.model.C
 
 import static software.amazon.cryptography.dbencryptionsdk.dynamodb.enhancedclient.DoNothingTag.CUSTOM_DDB_ENCRYPTION_DO_NOTHING_PREFIX;
 import static software.amazon.cryptography.dbencryptionsdk.dynamodb.enhancedclient.SignOnlyTag.CUSTOM_DDB_ENCRYPTION_SIGN_ONLY_PREFIX;
+import static software.amazon.cryptography.dbencryptionsdk.dynamodb.enhancedclient.SignAndIncludeInEncryptionContextTag.CUSTOM_DDB_ENCRYPTION_SIGN_AND_INCLUDE_PREFIX;
 
 public class DynamoDbEnhancedClientEncryption {
     public static DynamoDbEncryptionInterceptor CreateDynamoDbEncryptionInterceptor(
@@ -39,6 +41,7 @@ public class DynamoDbEnhancedClientEncryption {
                 .build();
     }
 
+    // return all attribute names that are keys in any index
     private static Set<String> attributeNamesUsedInIndices(
         final TableMetadata tableMetadata
     ) {
@@ -58,41 +61,95 @@ public class DynamoDbEnhancedClientEncryption {
         return allIndexAttributes;
     }
 
-    private static DynamoDbTableEncryptionConfig getTableConfig(
-        final DynamoDbEnhancedTableEncryptionConfig configWithSchema,
-        final String tableName
+    // return attributes used in the primary table index
+    private static Set<String> attributeNamesUsedInPrimaryKey(
+        final TableMetadata tableMetadata
     ) {
-        Map<String, CryptoAction> actions = new HashMap<>();
+        Set<String> keyAttributes = new HashSet<>();
+        tableMetadata.primaryKeys().stream()
+            .forEach(keyAttributes::add);
+        return keyAttributes;
+    }
 
-        TableSchema<?> topTableSchema = configWithSchema.schemaOnEncrypt();
+    private static void throwUsageError(String tableName, String attributeName, String usage, String usage2)
+    {
+        throw DynamoDbEncryptionException.builder()
+            .message(String.format(
+                "Attribute %s of table %s is used as both %s and %s.",
+                attributeName, tableName, usage, usage2))
+            .build();
+
+    }
+
+    // Any given attribute MUST have one and only one Cryptographic Action. 
+    // i.e: It can't be both SignOnly and DoNothing.
+    // validateAttributeUsage throws an error if 
+    // the given attribute is marked with `usage` and another Cryptographic Action.
+    // For example, for a SignOnly, signOnly will be empty, and an error must be reported
+    // if the attribute exists in any of the other sets.
+    private static void validateAttributeUsage(
+        String tableName,
+        String attributeName,
+        String usage,
+        Optional<Set<String>> signOnly,
+        Optional<Set<String>> signAndInclude,
+        Optional<Set<String>> doNothing
+    )
+    {
+        if (signOnly.isPresent()) {
+            if (signOnly.get().contains(attributeName)) {
+                throwUsageError(tableName, attributeName, usage, "@DynamoDbEncryptionSignOnly");
+            }
+        }
+        if (signAndInclude.isPresent()) {
+            if (signAndInclude.get().contains(attributeName)) {
+                throwUsageError(tableName, attributeName, usage, "@DynamoDbEncryptionSignAndIncludeInEncryptionContext");
+            }
+        }
+        if (doNothing.isPresent()) {
+            if (doNothing.get().contains(attributeName)) {
+                throwUsageError(tableName, attributeName, usage, "@DynamoDbEncryptionDoNothing");
+            }
+        }
+    }
+
+    // return a map containing all top level attributes in the schema
+    // If an attribute is used in an index, it is SignOnly
+    // Else if an attribute is tagged with a single action, it gets that action
+    // Else if an attribute is tagged with a multiple actions, an error is thrown
+    // Else if an attribute is not tagged, it is to be encrypted
+    private static Map<String, CryptoAction> getActionsFromSchema(String tableName, TableSchema<?> topTableSchema)
+    {
         Set<String> signOnlyAttributes = getSignOnlyAttributes(topTableSchema);
+        Set<String> signAndIncludeAttributes = getSignAndIncludeInEncryptionContextAttributes(topTableSchema);
         Set<String> doNothingAttributes = getDoNothingAttributes(topTableSchema);
         Set<String> keyAttributes = attributeNamesUsedInIndices(topTableSchema.tableMetadata());
-
-        if (!Collections.disjoint(keyAttributes, doNothingAttributes)) {
-            throw DynamoDbEncryptionException.builder()
-                    .message(String.format(
-                        "Cannot use @DynamoDbEncryptionDoNothing on primary key attributes. Found on Table Name: %s",
-                        tableName))
-                    .build();
-        } else if (!Collections.disjoint(signOnlyAttributes, doNothingAttributes)) {
-            throw DynamoDbEncryptionException.builder()
-                    .message(String.format(
-                        "Cannot use @DynamoDbEncryptionDoNothing and @DynamoDbEncryptionSignOnly on same attribute. Found on Table Name: %s",
-                        tableName))
-                    .build();
-        }
-
+        Set<String> tableKeys = attributeNamesUsedInPrimaryKey(topTableSchema.tableMetadata());
         List<String> attributeNames = topTableSchema.attributeNames();
+
+        Map<String, CryptoAction> actions = new HashMap<>();
         StringBuilder path = new StringBuilder();
         path.append(tableName).append(".");
         for (String attributeName : attributeNames) {
-            if (keyAttributes.contains(attributeName)) {
-                // key attributes are always SIGN_ONLY
-                actions.put(attributeName, CryptoAction.SIGN_ONLY);
+            if (tableKeys.contains(attributeName)) {
+                if (signAndIncludeAttributes.isEmpty()) {
+                    validateAttributeUsage(tableName, attributeName, "a primary key", Optional.empty(), Optional.of(signAndIncludeAttributes), Optional.of(doNothingAttributes));
+                    actions.put(attributeName, CryptoAction.SIGN_ONLY);
+                } else {
+                    validateAttributeUsage(tableName, attributeName, "a primary key", Optional.of(signOnlyAttributes), Optional.empty(), Optional.of(doNothingAttributes));
+                    actions.put(attributeName, CryptoAction.SIGN_AND_INCLUDE_IN_ENCRYPTION_CONTEXT);
+                }
             } else if (signOnlyAttributes.contains(attributeName)) {
+                validateAttributeUsage(tableName, attributeName, "@DynamoDbEncryptionSignOnly", Optional.empty(), Optional.of(signAndIncludeAttributes), Optional.of(doNothingAttributes));
+                actions.put(attributeName, CryptoAction.SIGN_ONLY);
+            } else if (signAndIncludeAttributes.contains(attributeName)) {
+                validateAttributeUsage(tableName, attributeName, "@DynamoDbEncryptionSignAndIncludeInEncryptionContext", Optional.of(signOnlyAttributes), Optional.empty(), Optional.of(doNothingAttributes));
+                actions.put(attributeName, CryptoAction.SIGN_AND_INCLUDE_IN_ENCRYPTION_CONTEXT);
+            } else if (keyAttributes.contains(attributeName)) {
+                validateAttributeUsage(tableName, attributeName, "an index key", Optional.empty(), Optional.of(signAndIncludeAttributes), Optional.of(doNothingAttributes));
                 actions.put(attributeName, CryptoAction.SIGN_ONLY);
             } else if (doNothingAttributes.contains(attributeName)) {
+                validateAttributeUsage(tableName, attributeName, "@DynamoDbEncryptionDoNothing", Optional.of(signOnlyAttributes), Optional.of(signAndIncludeAttributes), Optional.empty());
                 actions.put(attributeName, CryptoAction.DO_NOTHING);
             } else {
                 // non-key attributes are ENCRYPT_AND_SIGN unless otherwise annotated
@@ -102,12 +159,101 @@ public class DynamoDbEnhancedClientEncryption {
             // Detect Encryption Flags that are Ignored b/c they are in a Nested Class
             scanForIgnoredEncryptionTags(topTableSchema, attributeName, path);
         }
+        return actions;
+    }
+
+    // given action maps from multiple tables, merge them into one
+    // we throw an error if the one attribute is given two different actions
+    private static Map<String, CryptoAction> mergeActions(List<Map<String, CryptoAction>> actionList)
+    {
+        // most common case
+        if (actionList.size() == 1) {
+            return actionList.get(0);
+        }
+
+        // Gather set of all attributes
+        HashSet<String> attributes = new HashSet<>();
+        for (Map<String, CryptoAction> config : actionList) {
+            attributes.addAll(config.keySet());
+        }
+
+        // for each attribute, ensure that everyone agrees on its action
+        Map<String, CryptoAction> actions = new HashMap<>();
+        for (String attr : attributes) {
+            Optional<CryptoAction> action = Optional.empty();
+            for (Map<String, CryptoAction> config : actionList) {
+                CryptoAction act = config.get(attr);
+                if (act != null) {
+                    if (action.isPresent()) {
+                        if (!action.get().equals(act)) {
+                            throw DynamoDbEncryptionException.builder()
+                                .message(String.format(
+                                    "Attribute %s set to %s in one table and %s in another.",
+                                    attr, action.get(), act))
+                                .build();
+                        }
+                    } else {
+                        action = Optional.of(act);
+                    }
+                }
+            }
+            actions.put(attr, action.get());
+        }
+        return actions;
+    }
+
+    // return the partition key name
+    // throw an error if two schemas disagree
+    private static String getPartitionKeyName(List<TableSchema<?>> schemas)
+    {
+        String partitionName = schemas.get(0).tableMetadata().primaryPartitionKey();
+        for (TableSchema<?> schema : schemas) {
+            String part = schema.tableMetadata().primaryPartitionKey();
+            if (!partitionName.equals(part)) {
+                throw DynamoDbEncryptionException.builder()
+                    .message(String.format(
+                        "Primary Key set to %s in one table and %s in another.",
+                        partitionName, part))
+                    .build();
+            }
+        }
+        return partitionName;
+    }
+
+    // return the sort key name
+    // throw an error if two schemas disagree
+    private static Optional<String> getSortKeyName(List<TableSchema<?>> schemas)
+    {
+        Optional<String> sortName = schemas.get(0).tableMetadata().primarySortKey();
+        for (TableSchema<?> schema : schemas) {
+            Optional<String> sort = schema.tableMetadata().primarySortKey();
+            if (!sortName.equals(sort)) {
+                throw DynamoDbEncryptionException.builder()
+                    .message(String.format(
+                        "Primary Key set to %s in one table and %s in another.",
+                        sortName, sort))
+                    .build();
+            }
+        }
+        return sortName;
+    }
+
+    // Convert enhanced client config to regular config
+    private static DynamoDbTableEncryptionConfig getTableConfig(
+        final DynamoDbEnhancedTableEncryptionConfig configWithSchema,
+        final String tableName
+    ) {
+        List<Map<String, CryptoAction>> actionList = new ArrayList<>();
+        for (TableSchema<?> schema : configWithSchema.schemaOnEncrypt()) { 
+            actionList.add(getActionsFromSchema(tableName, schema));
+        }
+        Map<String, CryptoAction> actions = mergeActions(actionList);
 
         DynamoDbTableEncryptionConfig.Builder builder = DynamoDbTableEncryptionConfig.builder();
-        String partitionName = topTableSchema.tableMetadata().primaryPartitionKey();
+        String partitionName = getPartitionKeyName(configWithSchema.schemaOnEncrypt());
         builder = builder.partitionKeyName(partitionName);
 
-        Optional<String> sortName = topTableSchema.tableMetadata().primarySortKey();
+        Optional<String> sortName = getSortKeyName(configWithSchema.schemaOnEncrypt());
         if (sortName.isPresent()) {
             builder = builder.sortKeyName(sortName.get());
         }
@@ -139,6 +285,13 @@ public class DynamoDbEnhancedClientEncryption {
     private static Set<String> getSignOnlyAttributes(TableSchema<?> tableSchema) {
         return tableSchema.tableMetadata()
             .customMetadataObject(CUSTOM_DDB_ENCRYPTION_SIGN_ONLY_PREFIX, Set.class)
+            .orElseGet(HashSet::new);
+    }
+
+    @SuppressWarnings("unchecked")
+    private static Set<String> getSignAndIncludeInEncryptionContextAttributes(TableSchema<?> tableSchema) {
+        return tableSchema.tableMetadata()
+            .customMetadataObject(CUSTOM_DDB_ENCRYPTION_SIGN_AND_INCLUDE_PREFIX, Set.class)
             .orElseGet(HashSet::new);
     }
 
@@ -184,6 +337,16 @@ public class DynamoDbEnhancedClientEncryption {
                             "This is NOT Supported at this time!",
                         CUSTOM_DDB_ENCRYPTION_SIGN_ONLY_PREFIX,
                         attributePath.append(signOnlyAttributes.toArray()[0])))
+                    .build();
+            }
+            Set<String> signAndIncludeAttributes = getSignAndIncludeInEncryptionContextAttributes(subTableSchema);
+            if (signAndIncludeAttributes.size() > 0) {
+                throw DynamoDbEncryptionException.builder()
+                    .message(String.format(
+                        "Detected DynamoDbEncryption Tag %s on a nested attribute with Path %s. " +
+                            "This is NOT Supported at this time!",
+                        CUSTOM_DDB_ENCRYPTION_SIGN_AND_INCLUDE_PREFIX,
+                        attributePath.append(signAndIncludeAttributes.toArray()[0])))
                     .build();
             }
             Set<String> doNothingAttributes = getDoNothingAttributes(subTableSchema);
