DynamoDbEncryption/runtimes/java/src/main/smithy-generated/software/amazon/cryptography/dbencryptionsdk/dynamodb/itemencryptor/ToNative.java
@@ -147,6 +147,8 @@ public class ToNative {
     nativeBuilder.algorithmSuiteId(software.amazon.cryptography.materialproviders.ToNative.DBEAlgorithmSuiteId(dafnyValue.dtor_algorithmSuiteId()));
     nativeBuilder.encryptedDataKeys(software.amazon.cryptography.materialproviders.ToNative.EncryptedDataKeyList(dafnyValue.dtor_encryptedDataKeys()));
     nativeBuilder.storedEncryptionContext(software.amazon.cryptography.materialproviders.ToNative.EncryptionContext(dafnyValue.dtor_storedEncryptionContext()));
+    nativeBuilder.encryptionContext(software.amazon.cryptography.materialproviders.ToNative.EncryptionContext(dafnyValue.dtor_encryptionContext()));
+    nativeBuilder.selectorContext(software.amazon.cryptography.services.dynamodb.internaldafny.ToNative.Key(dafnyValue.dtor_selectorContext()));
     return nativeBuilder.build();
   }
 
