DynamoDbEncryption/runtimes/java/src/test/java/software/amazon/cryptography/dbencryptionsdk/dynamodb/enhancedclient/validdatamodels/SingleTable1.java
@@ -1,0 +1,123 @@
+package software.amazon.cryptography.dbencryptionsdk.dynamodb.enhancedclient.validdatamodels;
+
+import software.amazon.awssdk.enhanced.dynamodb.mapper.annotations.DynamoDbAttribute;
+import software.amazon.awssdk.enhanced.dynamodb.mapper.annotations.DynamoDbBean;
+import software.amazon.awssdk.enhanced.dynamodb.mapper.annotations.DynamoDbPartitionKey;
+import software.amazon.awssdk.enhanced.dynamodb.mapper.annotations.DynamoDbSortKey;
+import software.amazon.cryptography.dbencryptionsdk.dynamodb.enhancedclient.DynamoDbEncryptionDoNothing;
+import software.amazon.cryptography.dbencryptionsdk.dynamodb.enhancedclient.DynamoDbEncryptionSignOnly;
+import software.amazon.cryptography.dbencryptionsdk.dynamodb.enhancedclient.DynamoDbEncryptionSignAndIncludeInEncryptionContext;
+
+/**
+ * This class is used by the Enhanced Client Tests
+ */
+
+@DynamoDbBean
+public class SingleTable1 {
+
+    private String partitionKey;
+    private int sortKey;
+    private String encryptAndSign;
+    private String doNothing;
+    private String signOnly;
+
+    private String extraSignOnly1;
+    private String extraSignOnly12;
+    private String extraSignOnly13;
+    private String extraSignAndInclude1;
+    private String extraSignAndInclude12;
+    private String extraSignAndInclude13;
+    private String extraDoNothing1;
+    private String extraDoNothing12;
+    private String extraDoNothing13;
+    private String extraEncryptAndSign1;
+    private String extraEncryptAndSign12;
+    private String extraEncryptAndSign13;
+
+    public String getExtraEncryptAndSign1() {return this.extraEncryptAndSign1;}
+    public String getExtraEncryptAndSign12() {return this.extraEncryptAndSign12;}
+    public String getExtraEncryptAndSign13() {return this.extraEncryptAndSign13;}
+
+    @DynamoDbEncryptionDoNothing
+    public String getExtraDoNothing1() {return this.extraDoNothing1;}
+    @DynamoDbEncryptionDoNothing
+    public String getExtraDoNothing12() {return this.extraDoNothing12;}
+    @DynamoDbEncryptionDoNothing
+    public String getExtraDoNothing13() {return this.extraDoNothing13;}
+
+    @DynamoDbEncryptionSignOnly
+    public String getExtraSignOnly1() {return this.extraSignOnly1;}
+    @DynamoDbEncryptionSignOnly
+    public String getExtraSignOnly12() {return this.extraSignOnly12;}
+    @DynamoDbEncryptionSignOnly
+    public String getExtraSignOnly13() {return this.extraSignOnly13;}
+
+    @DynamoDbEncryptionSignAndIncludeInEncryptionContext
+    public String getExtraSignAndInclude1() {return this.extraSignAndInclude1;}
+    @DynamoDbEncryptionSignAndIncludeInEncryptionContext
+    public String getExtraSignAndInclude12() {return this.extraSignAndInclude12;}
+    @DynamoDbEncryptionSignAndIncludeInEncryptionContext
+    public String getExtraSignAndInclude13() {return this.extraSignAndInclude13;}
+
+    public void setExtraDoNothing1(String text) {this.extraDoNothing1 = text;}
+    public void setExtraDoNothing12(String text) {this.extraDoNothing12 = text;}
+    public void setExtraDoNothing13(String text) {this.extraDoNothing13 = text;}
+
+    public void setExtraSignOnly1(String text) {this.extraSignOnly1 = text;}
+    public void setExtraSignOnly12(String text) {this.extraSignOnly12 = text;}
+    public void setExtraSignOnly13(String text) {this.extraSignOnly13 = text;}
+
+    public void setExtraSignAndInclude1(String text) {this.extraSignAndInclude1 = text;}
+    public void setExtraSignAndInclude12(String text) {this.extraSignAndInclude12 = text;}
+    public void setExtraSignAndInclude13(String text) {this.extraSignAndInclude13 = text;}
+
+    public void setExtraEncryptAndSign1(String text) {this.extraEncryptAndSign1 = text;}
+    public void setExtraEncryptAndSign12(String text) {this.extraEncryptAndSign12 = text;}
+    public void setExtraEncryptAndSign13(String text) {this.extraEncryptAndSign13 = text;}
+
+    @DynamoDbPartitionKey
+    @DynamoDbAttribute(value = "partition_key")
+    public String getPartitionKey() {
+        return this.partitionKey;
+    }
+
+    public void setPartitionKey(String partitionKey) {
+        this.partitionKey = partitionKey;
+    }
+
+    @DynamoDbSortKey
+    @DynamoDbAttribute(value = "sort_key")
+    public int getSortKey() {
+        return this.sortKey;
+    }
+
+    public void setSortKey(int sortKey) {
+        this.sortKey = sortKey;
+    }
+
+    public String getEncryptAndSign() {
+        return this.encryptAndSign;
+    }
+
+    public void setEncryptAndSign(String encryptAndSign) {
+        this.encryptAndSign = encryptAndSign;
+    }
+
+    @DynamoDbEncryptionSignOnly
+    public String getSignOnly() {
+        return this.signOnly;
+    }
+
+    public void setSignOnly(String signOnly) {
+        this.signOnly = signOnly;
+    }
+
+    @DynamoDbEncryptionDoNothing
+    public String getDoNothing() {
+        return this.doNothing;
+    }
+
+    public void setDoNothing(String doNothing) {
+        this.doNothing = doNothing;
+    }
+}
