DynamoDbEncryption/runtimes/net/Generated/StructuredEncryption/ParsedHeader.cs
@@ -11,6 +11,7 @@ namespace AWS.Cryptography.DbEncryptionSDK.StructuredEncryption
     private AWS.Cryptography.MaterialProviders.DBEAlgorithmSuiteId _algorithmSuiteId;
     private System.Collections.Generic.List<AWS.Cryptography.MaterialProviders.EncryptedDataKey> _encryptedDataKeys;
     private System.Collections.Generic.Dictionary<string, string> _storedEncryptionContext;
+    private System.Collections.Generic.Dictionary<string, string> _encryptionContext;
     public AWS.Cryptography.DbEncryptionSDK.StructuredEncryption.CryptoSchema CryptoSchema
     {
       get { return this._cryptoSchema; }
@@ -47,12 +48,22 @@ namespace AWS.Cryptography.DbEncryptionSDK.StructuredEncryption
     {
       return this._storedEncryptionContext != null;
     }
+    public System.Collections.Generic.Dictionary<string, string> EncryptionContext
+    {
+      get { return this._encryptionContext; }
+      set { this._encryptionContext = value; }
+    }
+    public bool IsSetEncryptionContext()
+    {
+      return this._encryptionContext != null;
+    }
     public void Validate()
     {
       if (!IsSetCryptoSchema()) throw new System.ArgumentException("Missing value for required property 'CryptoSchema'");
       if (!IsSetAlgorithmSuiteId()) throw new System.ArgumentException("Missing value for required property 'AlgorithmSuiteId'");
       if (!IsSetEncryptedDataKeys()) throw new System.ArgumentException("Missing value for required property 'EncryptedDataKeys'");
       if (!IsSetStoredEncryptionContext()) throw new System.ArgumentException("Missing value for required property 'StoredEncryptionContext'");
+      if (!IsSetEncryptionContext()) throw new System.ArgumentException("Missing value for required property 'EncryptionContext'");
 
     }
   }
