DynamoDbEncryption/runtimes/net/Generated/StructuredEncryption/TypeConversion.cs
@@ -58,6 +58,7 @@ namespace AWS.Cryptography.DbEncryptionSDK.StructuredEncryption
     public static AWS.Cryptography.DbEncryptionSDK.StructuredEncryption.CryptoAction FromDafny_N3_aws__N12_cryptography__N15_dbEncryptionSdk__N20_structuredEncryption__S12_CryptoAction(software.amazon.cryptography.dbencryptionsdk.structuredencryption.internaldafny.types._ICryptoAction value)
     {
       if (value.is_ENCRYPT__AND__SIGN) return AWS.Cryptography.DbEncryptionSDK.StructuredEncryption.CryptoAction.ENCRYPT_AND_SIGN;
+      if (value.is_SIGN__AND__INCLUDE__IN__ENCRYPTION__CONTEXT) return AWS.Cryptography.DbEncryptionSDK.StructuredEncryption.CryptoAction.SIGN_AND_INCLUDE_IN_ENCRYPTION_CONTEXT;
       if (value.is_SIGN__ONLY) return AWS.Cryptography.DbEncryptionSDK.StructuredEncryption.CryptoAction.SIGN_ONLY;
       if (value.is_DO__NOTHING) return AWS.Cryptography.DbEncryptionSDK.StructuredEncryption.CryptoAction.DO_NOTHING;
       throw new System.ArgumentException("Invalid AWS.Cryptography.DbEncryptionSDK.StructuredEncryption.CryptoAction value");
@@ -65,6 +66,7 @@ namespace AWS.Cryptography.DbEncryptionSDK.StructuredEncryption
     public static software.amazon.cryptography.dbencryptionsdk.structuredencryption.internaldafny.types._ICryptoAction ToDafny_N3_aws__N12_cryptography__N15_dbEncryptionSdk__N20_structuredEncryption__S12_CryptoAction(AWS.Cryptography.DbEncryptionSDK.StructuredEncryption.CryptoAction value)
     {
       if (AWS.Cryptography.DbEncryptionSDK.StructuredEncryption.CryptoAction.ENCRYPT_AND_SIGN.Equals(value)) return software.amazon.cryptography.dbencryptionsdk.structuredencryption.internaldafny.types.CryptoAction.create_ENCRYPT__AND__SIGN();
+      if (AWS.Cryptography.DbEncryptionSDK.StructuredEncryption.CryptoAction.SIGN_AND_INCLUDE_IN_ENCRYPTION_CONTEXT.Equals(value)) return software.amazon.cryptography.dbencryptionsdk.structuredencryption.internaldafny.types.CryptoAction.create_SIGN__AND__INCLUDE__IN__ENCRYPTION__CONTEXT();
       if (AWS.Cryptography.DbEncryptionSDK.StructuredEncryption.CryptoAction.SIGN_ONLY.Equals(value)) return software.amazon.cryptography.dbencryptionsdk.structuredencryption.internaldafny.types.CryptoAction.create_SIGN__ONLY();
       if (AWS.Cryptography.DbEncryptionSDK.StructuredEncryption.CryptoAction.DO_NOTHING.Equals(value)) return software.amazon.cryptography.dbencryptionsdk.structuredencryption.internaldafny.types.CryptoAction.create_DO__NOTHING();
       throw new System.ArgumentException("Invalid AWS.Cryptography.DbEncryptionSDK.StructuredEncryption.CryptoAction value");
@@ -502,12 +504,13 @@ namespace AWS.Cryptography.DbEncryptionSDK.StructuredEncryption
       software.amazon.cryptography.dbencryptionsdk.structuredencryption.internaldafny.types.ParsedHeader concrete = (software.amazon.cryptography.dbencryptionsdk.structuredencryption.internaldafny.types.ParsedHeader)value; AWS.Cryptography.DbEncryptionSDK.StructuredEncryption.ParsedHeader converted = new AWS.Cryptography.DbEncryptionSDK.StructuredEncryption.ParsedHeader(); converted.CryptoSchema = (AWS.Cryptography.DbEncryptionSDK.StructuredEncryption.CryptoSchema)FromDafny_N3_aws__N12_cryptography__N15_dbEncryptionSdk__N20_structuredEncryption__S12_ParsedHeader__M12_cryptoSchema(concrete._cryptoSchema);
       converted.AlgorithmSuiteId = (AWS.Cryptography.MaterialProviders.DBEAlgorithmSuiteId)FromDafny_N3_aws__N12_cryptography__N15_dbEncryptionSdk__N20_structuredEncryption__S12_ParsedHeader__M16_algorithmSuiteId(concrete._algorithmSuiteId);
       converted.EncryptedDataKeys = (System.Collections.Generic.List<AWS.Cryptography.MaterialProviders.EncryptedDataKey>)FromDafny_N3_aws__N12_cryptography__N15_dbEncryptionSdk__N20_structuredEncryption__S12_ParsedHeader__M17_encryptedDataKeys(concrete._encryptedDataKeys);
-      converted.StoredEncryptionContext = (System.Collections.Generic.Dictionary<string, string>)FromDafny_N3_aws__N12_cryptography__N15_dbEncryptionSdk__N20_structuredEncryption__S12_ParsedHeader__M23_storedEncryptionContext(concrete._storedEncryptionContext); return converted;
+      converted.StoredEncryptionContext = (System.Collections.Generic.Dictionary<string, string>)FromDafny_N3_aws__N12_cryptography__N15_dbEncryptionSdk__N20_structuredEncryption__S12_ParsedHeader__M23_storedEncryptionContext(concrete._storedEncryptionContext);
+      converted.EncryptionContext = (System.Collections.Generic.Dictionary<string, string>)FromDafny_N3_aws__N12_cryptography__N15_dbEncryptionSdk__N20_structuredEncryption__S12_ParsedHeader__M17_encryptionContext(concrete._encryptionContext); return converted;
     }
     public static software.amazon.cryptography.dbencryptionsdk.structuredencryption.internaldafny.types._IParsedHeader ToDafny_N3_aws__N12_cryptography__N15_dbEncryptionSdk__N20_structuredEncryption__S12_ParsedHeader(AWS.Cryptography.DbEncryptionSDK.StructuredEncryption.ParsedHeader value)
     {
 
-      return new software.amazon.cryptography.dbencryptionsdk.structuredencryption.internaldafny.types.ParsedHeader(ToDafny_N3_aws__N12_cryptography__N15_dbEncryptionSdk__N20_structuredEncryption__S12_ParsedHeader__M12_cryptoSchema(value.CryptoSchema), ToDafny_N3_aws__N12_cryptography__N15_dbEncryptionSdk__N20_structuredEncryption__S12_ParsedHeader__M16_algorithmSuiteId(value.AlgorithmSuiteId), ToDafny_N3_aws__N12_cryptography__N15_dbEncryptionSdk__N20_structuredEncryption__S12_ParsedHeader__M17_encryptedDataKeys(value.EncryptedDataKeys), ToDafny_N3_aws__N12_cryptography__N15_dbEncryptionSdk__N20_structuredEncryption__S12_ParsedHeader__M23_storedEncryptionContext(value.StoredEncryptionContext));
+      return new software.amazon.cryptography.dbencryptionsdk.structuredencryption.internaldafny.types.ParsedHeader(ToDafny_N3_aws__N12_cryptography__N15_dbEncryptionSdk__N20_structuredEncryption__S12_ParsedHeader__M12_cryptoSchema(value.CryptoSchema), ToDafny_N3_aws__N12_cryptography__N15_dbEncryptionSdk__N20_structuredEncryption__S12_ParsedHeader__M16_algorithmSuiteId(value.AlgorithmSuiteId), ToDafny_N3_aws__N12_cryptography__N15_dbEncryptionSdk__N20_structuredEncryption__S12_ParsedHeader__M17_encryptedDataKeys(value.EncryptedDataKeys), ToDafny_N3_aws__N12_cryptography__N15_dbEncryptionSdk__N20_structuredEncryption__S12_ParsedHeader__M23_storedEncryptionContext(value.StoredEncryptionContext), ToDafny_N3_aws__N12_cryptography__N15_dbEncryptionSdk__N20_structuredEncryption__S12_ParsedHeader__M17_encryptionContext(value.EncryptionContext));
     }
     public static AWS.Cryptography.DbEncryptionSDK.StructuredEncryption.CryptoSchema FromDafny_N3_aws__N12_cryptography__N15_dbEncryptionSdk__N20_structuredEncryption__S12_CryptoSchema(software.amazon.cryptography.dbencryptionsdk.structuredencryption.internaldafny.types._ICryptoSchema value)
     {
@@ -684,6 +687,14 @@ namespace AWS.Cryptography.DbEncryptionSDK.StructuredEncryption
       return FromDafny_N3_aws__N12_cryptography__N17_materialProviders__S17_EncryptionContext(value);
     }
     public static Dafny.IMap<Dafny.ISequence<byte>, Dafny.ISequence<byte>> ToDafny_N3_aws__N12_cryptography__N15_dbEncryptionSdk__N20_structuredEncryption__S12_ParsedHeader__M23_storedEncryptionContext(System.Collections.Generic.Dictionary<string, string> value)
+    {
+      return ToDafny_N3_aws__N12_cryptography__N17_materialProviders__S17_EncryptionContext(value);
+    }
+    public static System.Collections.Generic.Dictionary<string, string> FromDafny_N3_aws__N12_cryptography__N15_dbEncryptionSdk__N20_structuredEncryption__S12_ParsedHeader__M17_encryptionContext(Dafny.IMap<Dafny.ISequence<byte>, Dafny.ISequence<byte>> value)
+    {
+      return FromDafny_N3_aws__N12_cryptography__N17_materialProviders__S17_EncryptionContext(value);
+    }
+    public static Dafny.IMap<Dafny.ISequence<byte>, Dafny.ISequence<byte>> ToDafny_N3_aws__N12_cryptography__N15_dbEncryptionSdk__N20_structuredEncryption__S12_ParsedHeader__M17_encryptionContext(System.Collections.Generic.Dictionary<string, string> value)
     {
       return ToDafny_N3_aws__N12_cryptography__N17_materialProviders__S17_EncryptionContext(value);
     }
