DynamoDbEncryption/dafny/DynamoDbEncryptionTransforms/Model/AwsCryptographyDbEncryptionSdkDynamoDbTransformsTypes.dfy
@@ -633,7 +633,7 @@ include "../../../../submodules/MaterialProviders/StandardLibrary/src/Index.dfy"
  datatype ResolveAttributesInput = | ResolveAttributesInput (
  nameonly TableName: ComAmazonawsDynamodbTypes.TableName ,
  nameonly Item: ComAmazonawsDynamodbTypes.AttributeMap ,
- nameonly Version: Option<AwsCryptographyDbEncryptionSdkDynamoDbTypes.VersionNumber>
+ nameonly Version: Option<AwsCryptographyDbEncryptionSdkDynamoDbTypes.VersionNumber> := Option.None
  )
  datatype ResolveAttributesOutput = | ResolveAttributesOutput (
  nameonly VirtualFields: StringMap ,
@@ -740,7 +740,7 @@ include "../../../../submodules/MaterialProviders/StandardLibrary/src/Index.dfy"
  import Operations : AbstractAwsCryptographyDbEncryptionSdkDynamoDbTransformsOperations
  function method DefaultDynamoDbTablesEncryptionConfig(): AwsCryptographyDbEncryptionSdkDynamoDbTypes.DynamoDbTablesEncryptionConfig
  method DynamoDbEncryptionTransforms(config: AwsCryptographyDbEncryptionSdkDynamoDbTypes.DynamoDbTablesEncryptionConfig := DefaultDynamoDbTablesEncryptionConfig())
- returns (res: Result<DynamoDbEncryptionTransformsClient, Error>)
+ returns (res: Result<IDynamoDbEncryptionTransformsClient, Error>)
 // BEGIN MANUAL EDIT
  requires var tmps0 := set t0 | t0 in config.tableEncryptionConfigs.Values;
  forall tmp0 :: tmp0 in tmps0 ==>
@@ -858,6 +858,13 @@ include "../../../../submodules/MaterialProviders/StandardLibrary/src/Index.dfy"
  tmp27.keyStore.ValidState()
 // END MANUAL EDIT
 
+ // Helper function for the benefit of native code to create a Success(client) without referring to Dafny internals
+ function method CreateSuccessOfClient(client: IDynamoDbEncryptionTransformsClient): Result<IDynamoDbEncryptionTransformsClient, Error> {
+   Success(client)
+ } // Helper function for the benefit of native code to create a Failure(error) without referring to Dafny internals
+ function method CreateFailureOfError(error: Error): Result<IDynamoDbEncryptionTransformsClient, Error> {
+   Failure(error)
+ }
  class DynamoDbEncryptionTransformsClient extends IDynamoDbEncryptionTransformsClient
  {
  constructor(config: Operations.InternalConfig)
