DynamoDbEncryption/dafny/DynamoDbItemEncryptor/src/Util.dfy
@@ -8,6 +8,12 @@ module DynamoDbItemEncryptorUtil {
   import opened Wrappers
   import opened StandardLibrary
   import opened StandardLibrary.UInt
+  import UTF8
+  import MPL = AwsCryptographyMaterialProvidersTypes
+  import DDB = ComAmazonawsDynamodbTypes
+  import SortedSets
+  import SE = StructuredEncryptionUtil
+  import DynamoToStruct
 
   const ReservedPrefix := "aws_dbe_"
   const BeaconPrefix := ReservedPrefix + "b_"
@@ -27,6 +33,197 @@ module DynamoDbItemEncryptorUtil {
   predicate method CharLess(x : char, y : char)
   {
     x < y
+  }
+
+  const TABLE_NAME : UTF8.ValidUTF8Bytes := UTF8.EncodeAscii("aws-crypto-table-name")
+  const PARTITION_NAME : UTF8.ValidUTF8Bytes := UTF8.EncodeAscii("aws-crypto-partition-name")
+  const SORT_NAME : UTF8.ValidUTF8Bytes := UTF8.EncodeAscii("aws-crypto-sort-name")
+
+  const SELECTOR_TABLE_NAME : DDB.AttributeName := "aws_dbe_table_name"
+  const SELECTOR_PARTITION_NAME : DDB.AttributeName := "aws_dbe_partition_name"
+  const SELECTOR_SORT_NAME : DDB.AttributeName := "aws_dbe_sort_name"
+
+  function method GetLiteralValue(x : seq<uint8>) : (ret : Result<DDB.AttributeValue, string>)
+  {
+    var str :- UTF8.Decode(x);
+    if str == SE.TRUE_STR then
+      Success(DDB.AttributeValue.BOOL(true))
+    else if str == SE.FALSE_STR then
+      Success(DDB.AttributeValue.BOOL(false))
+    else if str == SE.NULL_STR then
+      Success(DDB.AttributeValue.NULL(true))
+    else
+      Failure("Encryption Context literal value has unexpected value : '" + str + "'.")
+  }
+
+  function method GetSortKey(context : MPL.EncryptionContext) : Result<Option<UTF8.ValidUTF8Bytes>, string>
+  {
+    if SORT_NAME in context.Keys then
+      var sortName := SE.EC_ATTR_PREFIX + context[SORT_NAME];
+      :- Need(UTF8.ValidUTF8Seq(sortName), "Internal Error : bad utf8 in sortName");
+      Success(Some(sortName))
+    else
+      Success(None)
+  }
+
+  function method ConvertContextForSelector(context : MPL.EncryptionContext)
+    : (output: Result<DDB.Key, string>)
+    //= specification/dynamodb-encryption-client/ddb-encryption-branch-key-id-supplier.md#behavior
+    //= type=implication
+    //# - If the partition name does not exist in the encryption context, this operation MUST fail.
+    ensures PARTITION_NAME !in context.Keys ==> output.Failure?
+
+    ensures output.Success? ==>
+              //= specification/dynamodb-encryption-client/ddb-encryption-branch-key-id-supplier.md#behavior
+              //= type=implication
+              //# - It MUST deserialize the "aws-crypto-partition-name" value in the input encryption context to determine the partition name.
+              && PARTITION_NAME in context.Keys
+              && var partitionName := context[PARTITION_NAME];
+              && var partitionValueKey := SE.EC_ATTR_PREFIX + partitionName;
+              && partitionValueKey in context.Keys
+
+    //= specification/dynamodb-encryption-client/ddb-encryption-branch-key-id-supplier.md#behavior
+    //= type=implication
+    //# - It MUST get the serialized partition value by grabbing the `aws-crypto-attr.<partition_name>` from the encryption context.
+
+    //= specification/dynamodb-encryption-client/ddb-encryption-branch-key-id-supplier.md#behavior
+    //= type=implication
+    //# - If the partition value does not exist in the encryption context, this operation MUST fail.
+    ensures PARTITION_NAME in context.Keys ==>
+              && var partitionName := context[PARTITION_NAME];
+              && var partitionValueKey := SE.EC_ATTR_PREFIX + partitionName;
+              && (partitionValueKey !in context.Keys) ==> output.Failure?
+
+    //= specification/dynamodb-encryption-client/ddb-encryption-branch-key-id-supplier.md#behavior
+    //= type=implication
+    //# - It MUST check for the existence of "aws-crypto-sort-name" in the input encryption context.
+
+    //= specification/dynamodb-encryption-client/ddb-encryption-branch-key-id-supplier.md#behavior
+    //= type=implication
+    //# - If this key exists, it MUST get the serialized sort value by grabbing the `aws-crypto.attr:<sort_name>` from the encryption context.
+    ensures output.Success? && SORT_NAME in context.Keys ==>
+              && var sortName := context[SORT_NAME];
+              && var sortValueKey := SE.EC_ATTR_PREFIX + sortName;
+              && sortValueKey in context.Keys
+
+    //= specification/dynamodb-encryption-client/ddb-encryption-branch-key-id-supplier.md#behavior
+    //= type=implication
+    //# - If the sort value does not exist in the context, this operation MUST fail.
+    ensures SORT_NAME in context.Keys ==>
+              && var sortName := context[SORT_NAME];
+              && var sortValueKey := SE.EC_ATTR_PREFIX + sortName;
+              && (sortValueKey !in context.Keys ==> output.Failure?)
+  {
+    // Add partition key to map
+    :- Need(PARTITION_NAME in context.Keys, "Invalid encryption context: Missing partition name");
+    var partitionName := context[PARTITION_NAME];
+    var partitionValueKey := SE.EC_ATTR_PREFIX + partitionName;
+    :- Need(partitionValueKey in context.Keys, "Invalid encryption context: Missing partition value");
+
+    var sortValueKey :- GetSortKey(context);
+    :- Need(sortValueKey.None? || sortValueKey.value in context, "Invalid encryption context: Missing sort value");
+
+    var keys : seq<UTF8.ValidUTF8Bytes> := SortedSets.ComputeSetToOrderedSequence2(context.Keys, SE.ByteLess);
+
+    //= specification/dynamodb-encryption-client/ddb-encryption-branch-key-id-supplier.md#behavior
+    //# - If the field "aws-crypto-legend" exists in the encryption context,
+    //# it MUST [deserialize](./ddb-attribute-serialization.md), all values with keys beginning "aws-crypto-attr.",
+    //# and create a Key with these values, using names with the "aws-crypto-attr." removed.
+    if SE.LEGEND_UTF8 in context then
+      var legend :- UTF8.Decode(context[SE.LEGEND_UTF8]);
+      var attrMap :- GetV2AttrMap(keys, context, legend);
+
+      :- Need(TABLE_NAME in context, "Internal error, table name not in encryption context.");
+      var tableName :- UTF8.Decode(context[TABLE_NAME]);
+      var attrMap2 := attrMap[SELECTOR_TABLE_NAME := DDB.AttributeValue.S(tableName)];
+
+      :- Need(PARTITION_NAME in context, "Internal error, table name not in encryption context.");
+      var partitionName :- UTF8.Decode(context[PARTITION_NAME]);
+      var attrMap3 := attrMap2[SELECTOR_PARTITION_NAME := DDB.AttributeValue.S(partitionName)];
+
+      if SORT_NAME in context then
+        var sortName :- UTF8.Decode(context[SORT_NAME]);
+        Success(attrMap3[SELECTOR_SORT_NAME := DDB.AttributeValue.S(sortName)])
+      else
+        Success(attrMap3)
+
+    //= specification/dynamodb-encryption-client/ddb-encryption-branch-key-id-supplier.md#behavior
+    //# - If the field "aws-crypto-legend" does not exist in the encryption context, it MUST [deserialize the partition (and optionally sort) value](./ddb-attribute-serialization.md), and create a Key with these values.
+    else if sortValueKey.None? then
+      AddAttributeToMap(partitionValueKey, context[partitionValueKey], map[])
+    else
+      var attrMap :- AddAttributeToMap(partitionValueKey, context[partitionValueKey], map[]);
+      AddAttributeToMap(sortValueKey.value, context[sortValueKey.value], attrMap)
+  }
+
+  function method GetAttrValue(ecValue : UTF8.ValidUTF8Bytes, legend : char)
+    : Result<DDB.AttributeValue, string>
+  {
+    if legend == SE.LEGEND_STRING then
+      var value :- UTF8.Decode(ecValue);
+      Success(DDB.AttributeValue.S(value))
+    else if legend == SE.LEGEND_NUMBER then
+      var value :- UTF8.Decode(ecValue);
+      Success(DDB.AttributeValue.N(value))
+    else if legend == SE.LEGEND_LITERAL then
+      var value :- GetLiteralValue(ecValue);
+      Success(value)
+    else if legend == SE.LEGEND_BINARY then
+      var terminal :- SE.DecodeTerminal(ecValue);
+      var ddbAttrValue :- DynamoToStruct.BytesToAttr(terminal.value, terminal.typeId, false);
+      Success(ddbAttrValue.val)
+    else
+      Failure("Encryption Context Legend has unexpected character : '" + [legend] + "'.")
+  }
+
+  function method GetV2AttrMap(
+    keys : seq<UTF8.ValidUTF8Bytes>,
+    context : MPL.EncryptionContext,
+    legend : string,
+    attrMap : DDB.AttributeMap := map[]
+  )
+    : Result<DDB.AttributeMap, string>
+    requires forall k <- keys :: k in context
+  {
+    if |keys| == 0 then
+      if |legend| == 0 then
+        Success(attrMap)
+      else
+        Failure("Encryption Context Legend is too long.")
+    else
+      var key : UTF8.ValidUTF8Bytes := keys[0];
+      if SE.EC_ATTR_PREFIX < key then
+        :- Need(0 < |legend|, "Encryption Context Legend is too short.");
+        var attrName :- GetAttributeName(key);
+        var attrValue :- GetAttrValue(context[key], legend[0]);
+        GetV2AttrMap(keys[1..], context, legend[1..], attrMap[attrName := attrValue])
+      else
+        GetV2AttrMap(keys[1..], context, legend, attrMap)
+  }
+
+  function method GetAttributeName(ddbAttrKey: UTF8.ValidUTF8Bytes)
+    : (res: Result<DDB.AttributeName, string>)
+    requires |ddbAttrKey| >= |SE.EC_ATTR_PREFIX|
+  {
+    // Obtain attribute name from EC kvPair key
+    var ddbAttrNameBytes := ddbAttrKey[|SE.EC_ATTR_PREFIX|..];
+    var ddbAttrName :- UTF8.Decode(ddbAttrNameBytes);
+    :- Need(DDB.IsValid_AttributeName(ddbAttrName), "Invalid serialization of DDB Attribute in encryption context.");
+    Success(ddbAttrName)
+  }
+
+  function method AddAttributeToMap(ddbAttrKey: UTF8.ValidUTF8Bytes, encodedAttrValue: UTF8.ValidUTF8Bytes, attrMap: DDB.AttributeMap)
+    : (res: Result<DDB.AttributeMap, string>)
+    requires |ddbAttrKey| >= |SE.EC_ATTR_PREFIX|
+  {
+    var ddbAttrName :- GetAttributeName(ddbAttrKey);
+
+    // Obtain attribute value from EC kvPair value
+    var terminal :- SE.DecodeTerminal(encodedAttrValue);
+    var ddbAttrValue :- DynamoToStruct.BytesToAttr(terminal.value, terminal.typeId, false);
+
+    // Add to our AttributeMap
+    Success(attrMap[ddbAttrName := ddbAttrValue.val])
   }
 
 }
