DynamoDbEncryption/dafny/StructuredEncryption/Model/StructuredEncryption.smithy
@@ -45,6 +45,17 @@ operation DecryptStructure {
 @range(min:1, max:1)
 integer Version
 
+//= specification/structured-encryption/decrypt-structure.md#parsed-header
+//= type=implication
+//# This structure MUST contain the following values,
+//# representing the deserialized form of the header of the input encrypted structure:
+//#   - [Algorithm Suite ID](./header.md#format-flavor): The Algorithm Suite ID associated with the Format Flavor on the header.
+//#   - [Crypto Schema](./header.md#encrypt-legend): The Crypto Schema for each signed Terminal,
+//#     calculated using the Crypto Legend in the header, the signature scope used for decryption, and the data in the input structure.
+//#   - [Stored Encryption Context](./header.md#encryption-context): The Encryption Context stored in the header.
+//#   - [Encrypted Data Keys](./header.md#encrypted-data-keys): The Encrypted Data Keys stored in the header.
+//#   - [Encryption Context](#encryption-context): The full Encryption Context used.
+
 structure ParsedHeader {
     @required
     cryptoSchema: CryptoSchema,
@@ -53,7 +64,9 @@ structure ParsedHeader {
     @required
     encryptedDataKeys: EncryptedDataKeyList,
     @required
-    storedEncryptionContext: EncryptionContext
+    storedEncryptionContext: EncryptionContext,
+    @required
+    encryptionContext: EncryptionContext
 }
 
 structure EncryptStructureInput {
@@ -88,6 +101,11 @@ structure EncryptStructureInput {
     encryptionContext: EncryptionContext
 }
 
+//= specification/structured-encryption/encrypt-structure.md#output
+//= type=implication
+//# This operation MUST output the following:
+//# - [Encrypted Structured Data](#encrypted-structured-data)
+//# - [Parsed Header](./decrypt-structure.md#parsed-header)
 structure EncryptStructureOutput {
     @required
     encryptedStructure: StructuredData,
@@ -237,6 +255,10 @@ union CryptoSchemaContent {
     {
         "name": "ENCRYPT_AND_SIGN",
         "value": "ENCRYPT_AND_SIGN",
+    },
+    {
+        "name": "SIGN_AND_INCLUDE_IN_ENCRYPTION_CONTEXT",
+        "value": "SIGN_AND_INCLUDE_IN_ENCRYPTION_CONTEXT",
     },
     {
         "name": "SIGN_ONLY",
